Simplify a proof

Clean/Circomlib/AliasCheck.lean
@@ -50,11 +50,7 @@ def circuit {sentences : PropertySet (F p)} (order : SentenceOrder sentences) : 
     have : p > 2^135 := hp135.elim
     rcases h_holds with ⟨ h_holds1, h_holds3 ⟩
     simp only [h_holds3, h_input] at h_holds1
-    specialize h_holds1 (by
-      intros i x
-      specialize h_assumption i x
-      simp only [← h_input] at h_assumption
-      aesop)
+    specialize h_holds1 (by assumption)
     rcases h_holds1 with ⟨ h_holds11, h_holds12 ⟩
     split at h_holds12
     · aesop
